restructurization is in progress

core/scala/termware/src/main/scala/termware/ArrowTerm.scala
@@ -1,0 +1,70 @@
+package termware
+
+trait ArrowTerm extends PointTerm
+{
+  def left: MultiTerm
+  def right: MultiTerm
+
+  override def pointKind: PointKind = PointKind.Arrow(this)
+
+
+  override def uncontext: ArrowTerm with EmptyContext
+
+
+}
+
+
+trait ArrowTermImpl[S <: ArrowTermImpl[S]] extends ArrowTerm with PointTermImpl[S]
+{
+  this: S =>
+
+}
+
+
+case class DefaultArrowTerm(val left: MultiTerm, right: MultiTerm) extends ArrowTermImpl[DefaultArrowTerm] with EmptyContext
+{
+  override def name = ArrowName
+  override def arity: Int = 0
+
+  override def uncontext: ArrowTerm with EmptyContext = this
+  override def updateContext(ctx: MultiTerm): MultiTerm = ContextArrowTerm.create(this,ctx)
+
+  override def mergeAsLeftContext(other: MultiTerm): MultiTerm = ???
+
+  override def selectAsContextPattern(other: MultiTerm): MultiTerm = ???
+
+  override def mergeAsScopeAnd(other: MultiTerm): MultiTerm = ???
+
+  override def mergeAsScopeOr(other: MultiTerm): MultiTerm = ???
+
+  override def selectAsLeftPattern(other: MultiTerm): MultiTerm = ???
+}
+
+case class ContextArrowTerm(origin: ArrowTerm with EmptyContext, override val context:MultiTerm) extends ContextPointTerm(origin,context) with ArrowTermImpl[ContextArrowTerm]
+{
+  override def pointMergeAsLeftContext(other: PointTerm): MultiTerm = ???
+
+  override def left: MultiTerm = ContextMultiTerm.create(origin.left,context)
+
+  override def right: MultiTerm = ContextMultiTerm.create(origin.left,context)
+
+  override def uncontext: ArrowTerm with EmptyContext = origin
+
+}
+
+object ContextArrowTerm
+{
+
+  def create(a: ArrowTerm,context:MultiTerm):MultiTerm =
+    if (a.context.isEmpty) {
+      context.multiKind match {
+        case MultiKind.Empty(e) => a
+        case MultiKind.Error(e) => e
+        case MultiKind.Star(s) => create(a, s.context)
+        case _ => ContextArrowTerm(a.uncontext, context)
+      }
+    } else {
+      a.updateContext(context)
+    }
+
+}
