core/scala/termware/src/main/scala/termware/AtomTerm.scala
@@ -1,0 +1,53 @@
+package termware
+
+trait AtomTerm extends PointTerm
+{
+  def arity = 0
+
+  override def pointKind: PointKind = PointKind.Atom(this)
+}
+
+trait AtomTermImpl[S <: AtomTermImpl[S]] extends AtomTerm with PointTermImpl[S]
+{
+  this: S =>
+
+}
+
+case class DefaultAtomTerm(val name:Name) extends AtomTermImpl[DefaultAtomTerm] with EmptyContext
+{
+  override def pointKind: PointKind = PointKind.Atom(this)
+
+  override def updateContext(ctx: MultiTerm): MultiTerm =
+                                     ContextAtomTerm.create(this,ctx)
+
+  override def uncontext = this
+
+  override def mergeAsLeftContext(other: MultiTerm): MultiTerm = ???
+
+  override def selectAsContextPattern(other: MultiTerm): MultiTerm = ???
+
+  override def mergeAsScopeAnd(other: MultiTerm): MultiTerm = ???
+
+  override def mergeAsScopeOr(other: MultiTerm): MultiTerm = ???
+
+  override def selectAsLeftPattern(other: MultiTerm): MultiTerm = ???
+}
+
+case class ContextAtomTerm(origin:AtomTerm with EmptyContext, override val context: MultiTerm) extends ContextPointTerm(origin,context) with AtomTermImpl[ContextAtomTerm]
+{
+  override def arity = 0
+
+  override def pointMergeAsLeftContext(other: PointTerm): MultiTerm = ???
+
+  override def uncontext: AtomTerm with EmptyContext = origin
+}
+
+object ContextAtomTerm
+{
+  def create(a:AtomTerm,ctx:MultiTerm): MultiTerm =
+    ctx.multiKind match {
+      case MultiKind.Empty(e) => a
+      case MultiKind.Error(e) => e
+      case _ => ContextAtomTerm.create(a,ctx)
+    }
+}
