core/scala/termware/src/main/scala/termware/ContextTerm.scala
@@ -1,0 +1,157 @@
+package termware
+
+sealed trait ContextTerm
+
+abstract class ContextMultiTerm(origin:MultiTerm, context:MultiTerm) extends MultiTerm {
+
+  override def name: Name = origin.name
+
+  override def cardinality: Int = origin.cardinality
+
+  override def multiKind: MultiKind =
+     origin.multiKind match {
+       case x@MultiKind.Empty(e) => x
+       case x@MultiKind.Error(e) => x
+       case x@MultiKind.Star(s) =>
+                  s match {
+                    case DefaultStarTerm => MultiKind.Star(ContextStarTerm(context))
+                    case _ => ??? // impossible. If we have ContextStarTerm here, it means part of term come to us unnormalized
+                  }
+       case x@MultiKind.Set(s) => // impossible,
+                                  s.mapMerge(_.updateContext(context)).multiKind
+       case x@MultiKind.Point(pt) =>
+                          pt match {
+                            case ContextPointTerm(x,xc) => ??? //impossible()
+                            case _ => ContextPointTerm.create(pt,context).multiKind
+                          }
+
+     }
+
+
+}
+
+trait EmptyContext extends MultiTerm
+{
+  override def context: MultiTerm = EmptyTerm
+
+  override def uncontext: MultiTerm with EmptyContext = this
+}
+
+object ContextMultiTerm
+{
+
+  def create(v:MultiTerm, c:MultiTerm): MultiTerm =
+    v.multiKind match {
+      case MultiKind.Empty(e) => e
+      case MultiKind.Error(e) => e
+      case r =>
+        c.multiKind match {
+          case MultiKind.Empty(e) => v
+          case MultiKind.Error(e) => e
+          case _ =>
+            r match {
+              case MultiKind.Set(s) => s.mapMerge(_.updateContext(c))
+              case _ => ???
+            }
+        }
+
+    }
+
+}
+
+
+abstract class ContextPointTerm(pt:PointTerm,val context:MultiTerm) extends ContextMultiTerm(pt,context) with PointTerm
+{
+  override def arity: Int = pt.arity
+
+  override def name: Name = pt.name
+
+  override def updateContext(ctx: MultiTerm): MultiTerm =
+          ContextPointTerm.create(pt,ctx.mergeAsLeftContext(context))
+
+  override def mergeAsLeftContext(other: MultiTerm): MultiTerm =
+          other.multiKind match {
+            case MultiKind.Empty(e) => this
+            case MultiKind.Error(e) => e
+            case MultiKind.Set(s) => ???
+            case MultiKind.Point(pt) => if (pt == other) {
+              pt
+            } else {
+              pointMergeAsLeftContext(pt)
+            }
+            case MultiKind.Star(s) => this   // ??? !!
+          }
+
+  def pointMergeAsLeftContext(other: PointTerm): MultiTerm
+
+  override def selectAsContextPattern(other: MultiTerm): MultiTerm = ???
+
+  override def mergeAsScopeAnd(other: MultiTerm): MultiTerm = ???
+
+  override def mergeAsScopeOr(other: MultiTerm): MultiTerm = ???
+
+  override def selectAsLeftPattern(other: MultiTerm): MultiTerm = ???
+}
+
+object ContextPointTerm
+{
+
+  def create(pt: PointTerm,context: MultiTerm): MultiTerm =
+     pt.pointKind match {
+       case PointKind.Atom(a) => ContextAtomTerm.create(a,context)
+       case PointKind.Sequence(s) => ContextSequenceTerm.create(s,context)
+       case PointKind.Structured(s) => ContextStructuredTerm.create(s,context)
+       case PointKind.Arrow(s) => ContextArrowTerm.create(s,context)
+       case PointKind.Primitive(p) => p
+     }
+
+  def unapply(arg: PointTerm): Option[(PointTerm, MultiTerm)] =
+    arg.context match {
+      case EmptyTerm => None
+      case ctx => arg.pointKind match {
+        case PointKind.Primitive(p) => None
+        case PointKind.Arrow(a) => Some((a,ctx))
+        case PointKind.Atom(a) => Some((a,ctx))
+        case PointKind.Structured(s) => Some((s,ctx))
+        case PointKind.Sequence(s) => Some((s,ctx))
+      }
+    }
+
+}
+
+
+
+
+
+case class ContextStructuredTerm(origin: StructuredTerm with EmptyContext, override val context: MultiTerm) extends ContextPointTerm(origin,context) with StructuredTermImpl[ContextStructuredTerm]
+{
+  override def pointMergeAsLeftContext(other: PointTerm): MultiTerm = ???
+
+  override def get(n: Name): MultiTerm =
+     ContextMultiTerm.create(origin.get(n),context)
+
+  override def subterms(): IndexedSeq[MultiTerm] =
+      origin.subterms().map(ContextMultiTerm.create(_,context))
+
+  override def uncontext: StructuredTerm with EmptyContext = origin
+}
+
+object ContextStructuredTerm
+{
+
+  def create(origin: StructuredTerm, context:MultiTerm): MultiTerm =
+    context.multiKind match {
+      case MultiKind.Empty(e) => origin
+      case MultiKind.Error(e) => e
+      case x => if (origin.context.isEmpty) {
+        ContextStructuredTerm(origin.uncontext,context)
+      } else {
+        origin.updateContext(context)
+      }
+    }
+
+}
+
+
+
+
