core/scala/termware/src/main/scala/termware/EmptyTerm.scala
@@ -1,0 +1,29 @@
+package termware
+
+trait EmptyTerm extends MultiTerm
+
+
+case object EmptyTerm extends EmptyTerm {
+  override def name: Name = EmptyName
+
+  override def cardinality: Int = 0
+
+  override def multiKind: MultiKind = MultiKind.Empty(this)
+
+  override def context: MultiTerm = this
+
+  override def updateContext(ctx: MultiTerm): MultiTerm = ???
+
+  override def uncontext: MultiTerm with EmptyContext = ???
+
+  override def mergeAsLeftContext(other: MultiTerm): MultiTerm = ???
+
+  override def selectAsContextPattern(other: MultiTerm): MultiTerm = ???
+
+  override def mergeAsScopeAnd(other: MultiTerm): MultiTerm = ???
+
+  override def mergeAsScopeOr(other: MultiTerm): MultiTerm = ???
+
+  override def selectAsLeftPattern(other: MultiTerm): MultiTerm = ???
+}
+
