core/scala/termware/src/main/scala/termware/MultiKind.scala
@@ -1,0 +1,18 @@
+package termware
+
+/**
+  * trait for pattern matching over different variants of the MultiTerm.
+  */
+sealed trait MultiKind
+
+
+object MultiKind
+{
+
+  case class  Star(x:StarTerm) extends MultiKind
+  case class  Set(x:SetTerm) extends MultiKind
+  case class  Point(x:PointTerm) extends MultiKind
+  case class  Empty(x:EmptyTerm) extends MultiKind
+  case class  Error(x:ErrorTerm) extends MultiKind
+
+}
