core/scala/termware/src/main/scala/termware/MultiTerm.scala
@@ -1,319 +1,41 @@
 package termware
 
-sealed trait MergePolicy
-object MergePolicy
-{
-  case object LeftFirst extends MergePolicy
-  case object RightFirst extends MergePolicy
-  case object Unificate  extends MergePolicy
-  case object Disallow  extends MergePolicy
-}
-
-sealed trait MultiTerm
-{
+trait MultiTerm {
 
   def name: Name
-
   def cardinality: Int
+  def multiKind: MultiKind
 
-  def point(i:Int): Option[PointTerm]
-
-  def points: IndexedSeq[PointTerm]
-
-  def merge(x1: MultiTerm, mp: MergePolicy): MultiTerm
-    = operations.Merge(this,x1,mp)
-
-  def normalize(): MultiTerm = this
-
-}
-
-
-
-sealed trait PointTerm extends MultiTerm
-{
-  def name: Name
-
-  def cardinality: Int = 1
-
-  def point(i:Int): Option[PointTerm] =
-    i match {
-      case 0 => Some(this)
-      case _ => None
-    }
-
-  lazy val points: IndexedSeq[PointTerm] = IndexedSeq(this)
-
-  def arity: Int
-
-  def left: MultiTerm
-
-  def right: MultiTerm
-
-  def subterm(n:Name):Option[MultiTerm]
-
-  def subterm(i:Int):Option[MultiTerm]
-
-  def subterms(): IndexedSeq[MultiTerm]
-
-}
-
-sealed trait OrdinaryTerm extends PointTerm
-{
-  def left: MultiTerm = EmptyTerm
-  def right: MultiTerm = this
-
-  override def normalize() = this
-
-}
-
-sealed trait ZeroArityTerm extends OrdinaryTerm
-{
-  def name: Name
-
-  override def arity: Int = 0
-
-  override def subterm(i: Int): Option[MultiTerm] = None
-
-  override def subterm(n: Name): Option[MultiTerm] = None
-
-  override def subterms(): IndexedSeq[MultiTerm] = IndexedSeq.empty
-
-
-}
-
-class PrimiveTerm[T](val value:T, descriptor: PrimitiveDescriptor[T]) extends ZeroArityTerm
-{
-  override val name: Name = PrimitiveName(value)(descriptor)
-
-  override def normalize() = this
-}
-
-case class AtomTerm(override val name: Name) extends ZeroArityTerm
-{
-  override def arity: Int = 0
-  override def cardinality: Int = 1
-  override def normalize() = this
-}
-
-case class SequenceTerm(val values: IndexedSeq[MultiTerm]) extends OrdinaryTerm
-{
-  override def name = SequenceTerm.name
-  override def arity: Int = values.size
-
-  override def subterm(n: Name): Option[MultiTerm] = {
-    val i: Int = n.typeIndex match {
-      case IntPrimitiveDescriptor.primitiveTypeIndex => n.asInstanceOf[PrimitiveName[Int]].value
-      case BytePrimitiveDescriptor.primitiveTypeIndex => n.asInstanceOf[PrimitiveName[Byte]].value.toInt
-      case ShortPrimitiveDescriptor.primitiveTypeIndex => n.asInstanceOf[PrimitiveName[Short]].value.toInt
-      case _ => -1
-    }
-    subterm(i)
-  }
-
-  override def subterm(i: Int): Option[MultiTerm] =
-  {
-    if (i >= 0 && i < values.size) { // TODO, think how to eliminate in some cases
-      Some(values(i))
-    }else{
-      None
-    }
-  }
-
-  override def subterms(): IndexedSeq[MultiTerm] = values
-}
-
-object SequenceTerm
-{
-  final val name = SeqName
-}
-
-case class StructuredTerm(name:Name,values: NameIndexed[MultiTerm]) extends OrdinaryTerm
-{
-
-  override def arity = values.size
-
-  override def subterm(n: Name): Option[MultiTerm] = values.get(n)
-
-  override def subterm(i: Int): Option[MultiTerm] = values.get(i)
-
-  override def subterms(): IndexedSeq[MultiTerm] = values.values
-
-}
-
-final case class SetTerm(values: IndexedSeq[PointTerm]) extends MultiTerm
-{
-
-  override def name: Name = SetName
-
-  override def cardinality: Int = values.size
-
-  override def point(i: Int): Option[PointTerm] =
-    if (i >= 0 && i < values.size) {
-      Some(values(i))
-    } else {
-      None
-    }
-
-  override def points: IndexedSeq[PointTerm] = values
-
-  override def normalize():MultiTerm =
-  {
-    if (values.isEmpty)
-      EmptyTerm
-    else if (values.size == 1) {
-      values(0)
-    } else this
-  }
-
-}
-
-object SetTerm
-{
-  def create(values: IndexedSeq[PointTerm]): MultiTerm = {
-    if (values.isEmpty) {
-      EmptyTerm
-    } else if (values.size == 1) {
-      values(0)
-    } else {
-      new SetTerm(values)
-    }
-  }
-}
-
-sealed trait ScopedTerm extends MultiTerm
-{
-
-  this: MultiTerm =>
+  def isEmpty: Boolean  = this == EmptyTerm
 
   def context: MultiTerm
-}
+  def updateContext(ctx:MultiTerm): MultiTerm
+  def uncontext: MultiTerm with EmptyContext
 
-case class ScopedPointTerm(context: MultiTerm, body: PointTerm) extends PointTerm with ScopedTerm
-{
+  def mergeAsLeftContext(other: MultiTerm): MultiTerm
+  def mergeAsRightContext(other: MultiTerm): MultiTerm = other.mergeAsLeftContext(this)
 
-  override def cardinality: Int = body.cardinality
+  def selectAsContextPattern(other: MultiTerm): MultiTerm
+  def selectAgainstContextPattern(other: MultiTerm): MultiTerm = other.selectAsContextPattern(this)
 
-  override def name: Name = body.name
+  def mergeAsScopeAnd(other: MultiTerm):MultiTerm
+  def mergeAsScopeOr(other:MultiTerm): MultiTerm
 
-  override def point(i: Int): Option[PointTerm] =
-    body.point(i) map (t => ScopedPointTerm(context,t))
-
-  override lazy val points: IndexedSeq[PointTerm] =
-  {
-    body.points.map(p => ScopedPointTerm(context,p))
-  }
-
-  override def arity: Int = body.arity
-
-  override def left: MultiTerm = ScopedTerm(context,body.left)
-
-  override def right: MultiTerm = ScopedTerm(context,body.right)
-
-  override def subterm(n: Name): Option[MultiTerm] = body.subterm(n).map(ScopedTerm(context,_))
-
-  override def subterm(i: Int): Option[MultiTerm] = body.subterm(i).map(ScopedTerm(context,_))
-
-  override lazy val subterms: IndexedSeq[MultiTerm] =
-      body.subterms.map(ScopedTerm(context, _ ))
-
-  override def normalize(): MultiTerm = ScopedTerm(context,body)
+  def selectAsLeftPattern(other:MultiTerm):MultiTerm
 
 }
 
-case class  ScopedStarTerm(val context: MultiTerm) extends MultiTerm with ScopedTerm
-{
-  override def name: Name = StarTerm.name
 
-  override def cardinality: Int = StarTerm.cardinality
 
-  override def point(i: Int): Option[PointTerm] = StarTerm.point(i)
+trait MultiTermImpl[S <: MultiTermImpl[S]] extends MultiTerm {
 
-  override def points: IndexedSeq[PointTerm] = StarTerm.points
+    thisMultiTerm: S =>
+    //type D
+    type Self = S //<: MultiTerm.Aux[D]
 
-  override def normalize(): MultiTerm = this
-}
-
-case object ScopedTerm
-{
-
-  def apply(context:MultiTerm,body:MultiTerm):MultiTerm =
-  {
-    body match {
-      case SetTerm(values) => SetTerm(values.map(ScopedPointTerm(context,_)))
-      case ScopedTerm(context1,body) => ScopedTerm(context1.merge(context, MergePolicy.LeftFirst),body)
-      case EmptyTerm => EmptyTerm
-      case x: PointTerm => new ScopedPointTerm(context,x)
-      case e: ErrorTerm => e   // TODO: think
-      case StarTerm => ScopedStarTerm(context)
-    }
-  }
-
-  def unapply(arg: ScopedTerm): Option[(MultiTerm,MultiTerm)] =
-  {
-    arg match {
-      case ScopedStarTerm(context) => Some((context,StarTerm))
-      case ScopedPointTerm(context,body) => Some((context,body))
-    }
-  }
 
 }
 
-case class ArrowTerm(left: MultiTerm, right: MultiTerm) extends PointTerm
-{
-  override def name: Name = ArrowName
 
-  override def arity: Int = 2
 
-  override def subterm(n: Name): Option[MultiTerm] =
-  {
-    n match {
-      case StdNames.source => Some(left)
-      case StdNames.destination => Some(right)
-      case _ => None
-    }
-  }
 
-  override def subterm(i: Int): Option[MultiTerm] =
-    i match {
-      case 0 => Some(left)
-      case 1 => Some(right)
-      case _ => None
-    }
-
-  override def subterms(): IndexedSeq[MultiTerm] = IndexedSeq(left,right)
-}
-
-case object EmptyTerm extends MultiTerm
-{
-
-  override def name: Name = StarName
-
-  override def cardinality: Int = 0
-
-  override def points: IndexedSeq[PointTerm] = IndexedSeq.empty
-
-  override def point(i: Int): Option[PointTerm] = None
-
-}
-
-case object StarTerm extends MultiTerm
-{
-  override def name: Name = StarName
-
-  override def cardinality: Int = 0
-
-  override def point(i: Int): Option[PointTerm] = None
-
-  override def points: IndexedSeq[PointTerm] = IndexedSeq.empty
-}
-
-case class ErrorTerm(msg:String,ex:Option[Throwable], additional: MultiTerm) extends MultiTerm
-{
-  override def name: Name = ErrorName
-
-  override def cardinality: Int = 1
-
-  override def point(i: Int): Option[PointTerm] = None
-
-  override def points: IndexedSeq[PointTerm] = ???
-}
