core/scala/termware/src/main/scala/termware/PointTerm.scala
@@ -1,0 +1,25 @@
+package termware
+
+trait PointTerm extends MultiTerm {
+
+  def arity: Int
+
+  def pointKind: PointKind
+
+  override def uncontext: PointTerm with EmptyContext
+
+  override def cardinality: Int = 0
+
+  override def multiKind: MultiKind = MultiKind.Point(this)
+
+
+}
+
+
+trait PointTermImpl[S <: PointTermImpl[S]] extends PointTerm with MultiTermImpl[S] {
+
+  this : S =>
+
+}
+
+
