core/scala/termware/src/main/scala/termware/PrimitiveImplicits.scala
@@ -1,8 +1,0 @@
-package termware
-
-trait PrimitiveImplicits {
-
- implicit val intDescriptor : PrimitiveDescriptor[Int] = IntPrimitiveDescriptor
-
-
-}
