core/scala/termware/src/main/scala/termware/PrimitiveTerm.scala
@@ -1,0 +1,226 @@
+package termware
+
+
+
+trait PrimitiveTerm[T] extends PointTerm with EmptyContext
+{
+  def value:T
+
+  def primitiveTypeIndex: Int
+
+  def ordering: Ordering[T]
+
+  def termConstructor(x:T): PrimitiveTerm[T]
+
+  override def name: Name
+
+  override def arity: Int = 0
+
+  override def pointKind: PointKind = PointKind.Primitive(this)
+
+  override def context: MultiTerm = EmptyTerm
+
+  override def uncontext: PrimitiveTerm[T] with EmptyContext = this
+
+  override def updateContext(ctx: MultiTerm): MultiTerm = this
+
+  override def mergeAsLeftContext(other: MultiTerm): MultiTerm = ???
+
+  override def selectAsContextPattern(other: MultiTerm): MultiTerm = ???
+
+  override def mergeAsScopeAnd(other: MultiTerm): MultiTerm = ???
+
+  override def mergeAsScopeOr(other: MultiTerm): MultiTerm = ???
+
+  override def selectAsLeftPattern(other: MultiTerm): MultiTerm = ???
+
+
+}
+
+
+
+abstract class PrimitiveTermImpl[S<:PrimitiveTermImpl[S,T],T](val value: T) extends PrimitiveTerm[T] with PointTermImpl[S] {
+
+  this: S =>
+
+  override def name: Name = PrimitiveName(value)(ops)
+
+  def ops: PrimitiveTermOps[S,T]
+
+  def primitiveTypeIndex: Int = ops.primitiveTypeIndex
+
+  def ordering: Ordering[T] = ops.ordering
+
+  def termConstructor(x:T): PrimitiveTerm[T] = ops.termConstructor(x)
+
+
+}
+
+
+abstract class PrimitiveTermOps[S<:PrimitiveTermImpl[S,T],T]
+{
+
+  final type Primitive = T
+  type PName = PrimitiveName[T]
+
+  val primitiveTypeIndex: Int
+
+  def ordering: Ordering[T]
+
+  def termConstructor(x:T): PrimitiveTerm[T]
+
+
+}
+
+
+case class ByteTerm(v:Byte) extends PrimitiveTermImpl[ByteTerm,Byte](v)
+{
+  def ops = ByteTermOps
+
+}
+
+object ByteTermOps extends PrimitiveTermOps[ByteTerm,Byte]
+{
+
+  override final val primitiveTypeIndex: Int = 1
+
+  override def ordering: Ordering[Byte] = implicitly[Ordering[Byte]]
+
+  override def termConstructor(x: Byte): ByteTerm = ByteTerm(x)
+
+}
+
+case class ShortTerm(v:Short) extends PrimitiveTermImpl[ShortTerm,Short](v)
+{
+  def ops = ShortTermOps
+}
+
+object ShortTermOps extends PrimitiveTermOps[ShortTerm,Short]
+{
+  override final val primitiveTypeIndex: Int = 2
+
+  override def ordering: Ordering[Short] = implicitly[Ordering[Short]]
+
+  override def termConstructor(x: Short): ShortTerm = ShortTerm(x)
+
+}
+
+case class IntTerm(v:Int) extends PrimitiveTermImpl[IntTerm,Int](v)
+{
+  def ops = IntTermOps
+}
+
+object IntTermOps extends PrimitiveTermOps[IntTerm,Int]
+{
+  override final val primitiveTypeIndex: Int = 3
+
+  override def ordering: Ordering[Int] = implicitly[Ordering[Int]]
+
+  override def termConstructor(x: Int): IntTerm = IntTerm(x)
+}
+
+case class LongTerm(v:Long) extends PrimitiveTermImpl[LongTerm,Long](v)
+{
+  def ops = LongTermOps
+}
+
+
+object LongTermOps extends PrimitiveTermOps[LongTerm,Long]
+{
+  override final val primitiveTypeIndex: Int = 4
+
+  override def ordering: Ordering[Long] = implicitly[Ordering[Long]]
+
+  override def termConstructor(x: Long): LongTerm = LongTerm(x)
+}
+
+case class DoubleTerm(v:Double) extends PrimitiveTermImpl[DoubleTerm,Double](v)
+{
+  def ops = DoubleTermOps
+}
+
+
+object DoubleTermOps extends PrimitiveTermOps[DoubleTerm,Double]
+{
+  override val primitiveTypeIndex: Int = 8
+
+  override def ordering: Ordering[Double] = implicitly[Ordering[Double]]
+
+  override def termConstructor(x: Double): DoubleTerm = DoubleTerm(x)
+}
+
+case class BigDecimalTerm(v:BigDecimal) extends PrimitiveTermImpl[BigDecimalTerm,BigDecimal](v)
+{
+  def ops = BigDecimalTermOps
+}
+
+object BigDecimalTermOps extends PrimitiveTermOps[BigDecimalTerm,BigDecimal]
+{
+  override val primitiveTypeIndex: Int = 9
+
+  override def ordering: Ordering[BigDecimal] = implicitly[Ordering[BigDecimal]]
+
+  override def termConstructor(x: BigDecimal) = BigDecimalTerm(x)
+}
+
+//TODO: add unsigned types
+
+
+case class CharTerm(v:Char) extends PrimitiveTermImpl[CharTerm,Char](v)
+{
+  def ops = CharTermOps
+}
+
+
+object CharTermOps extends PrimitiveTermOps[CharTerm,Char]
+{
+  override final val primitiveTypeIndex: Int = 17
+
+  override def ordering: Ordering[Char] = implicitly[Ordering[Char]]
+
+  override def termConstructor(x: Char): CharTerm = CharTerm(x)
+}
+
+
+case class StringTerm(v:String) extends PrimitiveTermImpl[StringTerm,String](v)
+{
+  def ops = StringTermOps
+}
+
+
+object StringTermOps extends PrimitiveTermOps[StringTerm,String]
+{
+  override final val primitiveTypeIndex: Int = 18
+
+  override def ordering: Ordering[String] = implicitly[Ordering[String]]
+
+  override def termConstructor(x: String) = StringTerm(x)
+}
+
+case class OpaqueTerm(v:Array[Byte]) extends PrimitiveTermImpl[OpaqueTerm,Array[Byte]](v)
+{
+  def ops = OpaqueTermOps
+}
+
+object OpaqueTermOps extends PrimitiveTermOps[OpaqueTerm,Array[Byte]]
+{
+
+  override final val primitiveTypeIndex: Int = 19
+
+  override val ordering: Ordering[Array[Byte]] = (x: Array[Byte], y: Array[Byte]) => {
+    val c0 = x.length - y.length
+    if (c0 != 0) {
+      c0
+    } else {
+      var i = 0
+      var c = 0
+      while (i < x.length && c != 0) {
+        c = x(i) - y(i)
+        i += 1
+      }
+      c
+    }
+  }
+
+  override def termConstructor(x: Array[Byte]) = OpaqueTerm(x)
+}
