core/scala/termware/src/main/scala/termware/SequenceTerm.scala
@@ -1,0 +1,61 @@
+package termware
+
+
+trait SequenceTerm extends PointTerm {
+
+  def subterm(i:Int): MultiTerm
+
+  def subterms(): IndexedSeq[MultiTerm]
+
+  override def pointKind: PointKind = PointKind.Sequence(this)
+
+  override def uncontext: SequenceTerm with EmptyContext
+
+  override def name: Name = SeqName
+
+}
+
+trait SequenceTermImpl[S<:SequenceTermImpl[S]] extends SequenceTerm with PointTermImpl[S]
+{
+  this: S =>
+
+}
+
+case class DefaultSequenceTerm(values:IndexedSeq[MultiTerm]) extends SequenceTermImpl[DefaultSequenceTerm]
+{
+  override def subterm(i: Int): MultiTerm = ???
+
+  override def subterms(): IndexedSeq[MultiTerm] = ???
+
+  override def arity: Int = ???
+
+  override def context: MultiTerm = ???
+
+}
+
+
+case class ContextSequenceTerm(origin: SequenceTerm with EmptyContext, override val context: MultiTerm) extends ContextPointTerm(origin, context) with SequenceTermImpl[ContextSequenceTerm]
+{
+  override def subterm(i: Int): MultiTerm =
+    ContextMultiTerm.create(origin.subterm(i),context)
+
+  override def subterms(): IndexedSeq[MultiTerm] =
+    origin.subterms().map(ContextMultiTerm.create(_,context))
+
+
+}
+
+
+object ContextSequenceTerm
+{
+  def create(origin: SequenceTerm, ctx:MultiTerm):MultiTerm =
+    ctx.multiKind match {
+      case MultiKind.Empty(e) => origin
+      case MultiKind.Error(e) => e
+      case _ => if (origin.context.isEmpty) {
+        ContextSequenceTerm(origin.uncontext,ctx)
+      } else {
+        origin.updateContext(ctx)
+      }
+    }
+}
