core/scala/termware/src/main/scala/termware/SetTerm.scala
@@ -1,0 +1,38 @@
+package termware
+
+trait SetTerm extends MultiTerm {
+
+  override def name: Name = SetName
+
+  override def multiKind: MultiKind = MultiKind.Set(this)
+
+  def mapMerge(f:MultiTerm => MultiTerm): MultiTerm
+
+}
+
+trait SetTermImpl[S <: SetTermImpl[S]] extends SetTerm with MultiTermImpl[S]
+{
+  this: S =>
+
+
+}
+
+case class DefaultSetTerm(data:NameIndexed[PointTerm]) extends SetTermImpl[DefaultSetTerm]
+{
+
+  override def mapMerge(f: (MultiTerm) => MultiTerm): Unit = ???
+
+  override def cardinality: Int = data.size
+
+  override def multiKind: MultiKind = ???
+
+  override def select(pattern: MultiTerm): MultiTerm = ???
+
+  override def context: MultiTerm = ???
+
+  override def contextOr(otherContext: MultiTerm): MultiTerm = ???
+
+  override def contextAnd(otherContext: MultiTerm): MultiTerm = ???
+}
+
+
