core/scala/termware/src/main/scala/termware/StarTerm.scala
@@ -1,0 +1,65 @@
+package termware
+
+
+trait StarTerm extends MultiTerm
+{
+  override def name: Name = StarName
+
+  override def cardinality: Int = Int.MaxValue
+
+  override def multiKind: MultiKind = MultiKind.Star(this)
+
+
+}
+
+
+/**
+  * Plain Star term without context.
+  */
+case object DefaultStarTerm extends StarTerm with EmptyContext {
+
+  override def context: MultiTerm = EmptyTerm
+
+  override def updateContext(ctx: MultiTerm): MultiTerm =
+      ctx.multiKind match {
+        case MultiKind.Star(x) => ???
+        case MultiKind.Error(e) => e
+        case MultiKind.Empty(e) => this
+        case MultiKind.Set(e) => ContextStarTerm(e)
+        case MultiKind.Point(p) => ContextStarTerm(p)
+      }
+
+
+}
+
+case class ContextStarTerm(context:MultiTerm) extends  ContextMultiTerm(DefaultStarTerm,context) with StarTerm with MultiTermImpl[ContextStarTerm]
+{
+  override def updateContext(ctx: MultiTerm): MultiTerm =
+    ctx.multiKind match {
+      case MultiKind.Empty(e) => this
+      case MultiKind.Error(e) => e
+      case r => ContextStarTerm.create(ctx.mergeAsLeftContext(context))
+    }
+
+  override def uncontext: MultiTerm with EmptyContext = DefaultStarTerm
+
+  override def mergeAsLeftContext(other: MultiTerm): MultiTerm = ???
+
+  override def selectAsContextPattern(other: MultiTerm): MultiTerm = ???
+
+  override def mergeAsScopeAnd(other: MultiTerm): MultiTerm = ???
+
+  override def mergeAsScopeOr(other: MultiTerm): MultiTerm = ???
+
+  override def selectAsLeftPattern(other: MultiTerm): MultiTerm = ???
+}
+
+object ContextStarTerm
+{
+  def create(ctx:MultiTerm):MultiTerm =
+    ctx.multiKind match {
+      case MultiKind.Empty(e) => DefaultStarTerm
+      case MultiKind.Error(e) => e
+      case _ => ContextStarTerm(ctx)
+    }
+}
