core/scala/termware/src/main/scala/termware/StructuredTerm.scala
@@ -1,0 +1,25 @@
+package termware
+
+trait StructuredTerm extends PointTerm
+{
+
+  def get(n:Name): MultiTerm
+
+  def subterms():IndexedSeq[MultiTerm]
+
+  override def pointKind: PointKind = PointKind.Structured(this)
+
+  override def uncontext: StructuredTerm with EmptyContext
+
+}
+
+trait StructuredTermImpl[S <: StructuredTermImpl[S]] extends StructuredTerm with PointTermImpl[S] {
+
+  this: S =>
+
+
+}
+
+case class DefaultStructuredTerm(indexes:NameIndexed[MultiTerm])
+
+
