core/scala/termware/src/main/scala/termware/TermLanguage.scala
@@ -1,0 +1,14 @@
+package termware
+
+
+import scala.language.higherKinds
+
+trait TermLanguage {
+
+   def name: AtomTerm
+
+   def typer: TermTransformer
+
+   def interpreter: TermTransformer
+
+}
