core/scala/termware/src/main/scala/termware/TermMapping.scala
@@ -1,0 +1,13 @@
+package termware
+
+
+import scala.util.Try
+
+trait TermMapping[T]
+{
+
+  def toScala(x:MultiTerm):Try[T]
+
+  def fromScala(x:T):Try[MultiTerm]
+
+}
