core/scala/termware/src/main/scala/termware/TermTransformer.scala
@@ -1,0 +1,13 @@
+package termware
+
+import cats.effect.Effect
+
+import scala.language.higherKinds
+
+trait TermTransformer {
+
+
+    def transform[Eff[_]](x:Eff[MultiTerm])(implicit effect:Effect[Eff]): Eff[MultiTerm]
+
+
+}
