core/scala/termware/src/main/scala/termware/operations/ContextOr.scala
@@ -1,0 +1,9 @@
+package termware.operations
+
+import termware.MultiTerm
+
+object ContextOr {
+
+
+
+}
