core/scala/termware/src/main/scala/termware/operations/PointTermEq.scala
@@ -1,0 +1,12 @@
+package termware.operations
+
+import cats.Eq
+import termware.PointTerm
+
+object PointTermEq extends Eq[PointTerm] {
+
+  override def eqv(x: PointTerm, y: PointTerm): Boolean = ???
+
+}
+
+
