core/scala/termware/src/main/scala/termware/operations/ScopeAnd.scala
@@ -1,0 +1,19 @@
+package termware.operations
+
+import cats.effect.Effect
+import termware.{MultiTerm, PointTerm}
+import termware.plain._
+
+object ScopeAnd  {
+
+
+    def apply(x: MultiTerm, y: MultiTerm): MultiTerm = ???
+
+
+
+    def applyPointSet(x:PointTerm, y: IndexedSeq[PointTerm]): PointTerm = ???
+
+
+
+
+}
