core/scala/termware/src/main/scala/termware/operations/ScopeOr.scala
@@ -1,0 +1,8 @@
+package termware.operations
+
+/**
+  * Created by rssh on 8/27/17.
+  */
+class ScopeOr {
+
+}
