core/scala/termware/src/main/scala/termware/package.scala
@@ -1,0 +1,21 @@
+import termware.plain._
+
+import scala.language.implicitConversions
+
+
+package object termware  {
+
+  implicit def byteToTerm(b:Byte): ByteTerm = ByteTerm(b)
+
+  implicit def charToTerm(ch:Char): CharTerm = CharTerm(ch)
+
+  implicit def intToTerm(v:Int): IntTerm = IntTerm(v)
+
+  implicit def bigDecimalToTerm(v:BigDecimal): BigDecimalTerm = BigDecimalTerm(v)
+
+  implicit def stringToTerm(s:String): StringTerm = StringTerm(s)
+
+
+
+
+}
