core/scala/termware/src/main/scala/termware/scalastd.scala
@@ -1,0 +1,13 @@
+package termware
+
+import com.sun.xml.internal.xsom.impl.Ref.Term
+
+import scala.util.Try
+
+/**
+  * Representation of standard scala constructs.
+  */
+trait scalastd {
+
+
+}
