core/coq/Base.v
@@ -4,6 +4,7 @@ Require Import Ascii.
 Require Import String.
 Require Import List.
 Require Import FSets.FMapAVL.
+Require Import Coq.Lists.ListSet.
 Require Import Coq.Structures.OrderedTypeEx.
 
 Set Implicit Arguments.
@@ -18,45 +19,348 @@ Inductive PrimitiveValue :=
  | StringTerm: string -> PrimitiveValue .
 
 
+Lemma PrimitiveValue_eq_dec: forall x y:PrimitiveValue, { x = y} + { x <> y}.
+ decide equality.
+apply eq_nat_dec.
+apply bool_dec.
+apply string_dec.
+Defined.
+
+Fixpoint PrimitiveValue_eqb (x:PrimitiveValue) (y :PrimitiveValue): bool :=
+  if (PrimitiveValue_eq_dec x y) then true else false
+.
+
+
 Inductive Name : Set := 
    PrimitiveName: PrimitiveValue-> Name
  | StringName: string -> Name
  | SeqName  .
 
+
+Lemma Name_eq_dec: forall x y: Name, { x = y} + { x <> y}.
+ decide equality.
+ apply PrimitiveValue_eq_dec.
+ apply string_dec.
+Defined.
+
+
 (* Module Map_Name := FMapAVL.Make Name. *)
 
 
-
-Inductive PointTerm: Set := 
+Inductive PointTerm:Type := 
     primitiveTerm : PrimitiveValue -> PointTerm
   |  atomTerm:  Name -> PointTerm
   |  sequenceTerm:  (list MultiTerm) -> PointTerm
-  |  structuredTerm: (list (Name->MultiTerm)) -> PointTerm
+  |  structuredTerm: (list (Name * MultiTerm)) -> PointTerm
   |  scopedPointTerm: MultiTerm -> PointTerm -> PointTerm
   |  arrowTerm: MultiTerm -> MultiTerm -> PointTerm
-with MultiTerm: Set :=
+  |  nilTerm
+with MultiTerm:Type :=
    point: PointTerm -> MultiTerm
- | setTerm:  (list PointTerm) -> MultiTerm
+ | setTerm:  (set PointTerm) -> MultiTerm
  | scopedStarTerm: MultiTerm -> MultiTerm 
  | starTerm: MultiTerm
  | errorTerm: string -> MultiTerm
 .
 
+Lemma pair_eq_dec :
+  forall (A B:Type) (* should be Type in coq >= V8.1 *)
+         (eqA:forall a a0:A, {a=a0}+{a<>a0})
+         (eqB:forall b b0:B, {b=b0}+{b<>b0})
+         (x y:A*B), {x=y}+{x<>y}.
+Proof. intros until 2; decide equality; auto. Qed.
 
-Definition EmptyTerm := setTerm nil
-.
+
+Definition EmptyTerm := setTerm nil.
+
+Lemma Atom_eq_dec: forall (nx: Name)(ny: Name), {(atomTerm nx)=(atomTerm ny)} + {(atomTerm nx)<>(atomTerm ny)}.
+ intros.
+assert ( {nx = ny} + {nx <> ny}).
+apply Name_eq_dec.
+destruct H as [|e'].
+- rewrite e.
+  left.
+  congruence.
+- right.
+  congruence.
+Qed.
+
+Lemma Primitive_eq_dec: forall(px:PrimitiveValue)(py:PrimitiveValue), {(primitiveTerm px)=(primitiveTerm py)} + {(primitiveTerm px)<>(primitiveTerm py)}.
+intros.
+assert ({px = py} + {px <> py}).
+apply PrimitiveValue_eq_dec.
+destruct H as [|ne].
+  left; congruence.
+  right; congruence.
+Qed.
 
 Definition AtomTerm (x:Name)  := point (atomTerm x).
 Definition SequenceTerm (x: list MultiTerm) := point (sequenceTerm x).
 
 
+Lemma  seq_dec_eq_prop: forall x y, ( {x=y} + { x<>y } ) -> { (sequenceTerm x) = (sequenceTerm y)} + { (sequenceTerm x) <>  (sequenceTerm y)}.
+intros.
+case H as [E|NE].
+left; congruence.
+right; congruence.
+Qed.
+
+Lemma fin_list_nonrec: forall A (l: list A) (a:A), l<>a::l.
+ induction l.
+ - discriminate.
+ - injection 1.
+intros H0 _; now destruct (IHl a).
+Qed.
+
+Lemma  mt_pt_dec_prop: (forall x y: MultiTerm, { x = y} + { x <> y}) -> forall z v:PointTerm, { z = v } + { z <> v }.
+Proof.
+decide equality.
+apply PrimitiveValue_eq_dec.
+apply Name_eq_dec.
+apply list_eq_dec.
+apply X.
+apply list_eq_dec.
+apply pair_eq_dec.
+apply Name_eq_dec.
+apply X.
+Qed.
+
+Lemma  pt_mt_dec_prop: (forall x y: PointTerm, { x = y} + { x <> y}) -> forall z v:MultiTerm, { z = v } + { z <> v }.
+
+Proof.
+decide equality.
+apply list_eq_dec.
+apply X.
+apply string_dec.
+Qed.
+
+Print PointTerm_ind.
+
+
+Fixpoint PointTermDepth (x:PointTerm): nat :=
+  match x with 
+    primitiveTerm v  => 1
+  |  atomTerm n => 1
+  | sequenceTerm ls  =>  (fold_left (fun s e => 
+                                                            (max s (MultiTermDepth e))) ls 1) + 1 
+  | structuredTerm ls => (fold_left ( fun s e =>
+                                                          ( max s (MultiTermDepth (snd e) ))  ) ls 1 ) + 1
+ | scopedPointTerm mt pt => (max (MultiTermDepth mt) (PointTermDepth pt)  ) + 1
+ | arrowTerm mx my => (max  (MultiTermDepth mx) (MultiTermDepth my)  ) + 1 
+ | nilTerm => 0
+  end with MultiTermDepth (x: MultiTerm): nat :=
+   match x with
+     point y => (PointTermDepth y) + 1
+   | setTerm sp => (fold_left (fun s e => max s (PointTermDepth e)) sp 1 )+1
+   | scopedStarTerm mt => (MultiTermDepth mt)+1
+   | starTerm => 0
+   | errorTerm s => 0
+   end. 
+
+Lemma  nat_plus1_neq0: forall x: nat, x+1 <> 0.
+Proof.
+ intuition.
+Qed.
+
+Lemma PointTermDepth_0:  forall x:PointTerm, (PointTermDepth x) = 0 -> x = nilTerm.
+ intros.
+ induction (x).
+- compute in H.
+ + discriminate (H).
+- compute in H.
+ + discriminate H.
+- unfold  PointTermDepth in H.
+  apply nat_plus1_neq0 in H.
+  destruct H.
+- unfold  PointTermDepth in H.
+  apply nat_plus1_neq0 in H.
+  destruct H.
+- unfold  PointTermDepth in H.
+  apply nat_plus1_neq0 in H.
+  destruct H.
+- unfold  PointTermDepth in H.
+  apply nat_plus1_neq0 in H.
+  destruct H.
+- reflexivity.
+ Qed.
+
+
+Lemma MultiTermDepth_0:  forall x:MultiTerm, (MultiTermDepth x) = 0 -> { x = starTerm } + { exists s:string, x = (errorTerm s) }  .
+ intros.
+ remember x as y.
+ induction y.
+- unfold  MultiTermDepth in H.
+  apply nat_plus1_neq0 in H.
+  destruct H.
+- compute in H.
+  apply nat_plus1_neq0 in H.
+  destruct H.
+- unfold  MultiTermDepth in H.
+  apply nat_plus1_neq0 in H.
+  destruct H.
+- unfold  MultiTermDepth in H.
+  auto.
+- right.
+  exists s.
+  congruence.
+Qed.
+
+Lemma MaxAA: forall a: nat, (max a a) = a.
+intro.
+unfold max.
+induction a.
+auto.
+congruence.
+Qed.
+
+Lemma MaxL: forall a b:nat, (max a b) >= a.
+intros.
+induction a.
+- unfold max.
+  { induction b.
+    - auto.
+    - auto.
+  }
+- induction b.
+  auto.
+  simpl.
+  
+ 
+Qed.
+
+Lemma SeqDepthStep: forall (x:PointTerm) (yh: MultiTerm) (yt: list MultiTerm), x = sequenceTerm (yh::yt) -> (PointTermDepth x) > (MultiTermDepth yh).
+Proof.
+ intros.
+ subst x.
+ unfold PointTermDepth. 
+
+Qed.  
+
+
+Lemma unnorm_pointterm_eq_dec: forall x: PointTerm, forall y: PointTerm, { x = y } + {  x <> y }.
+Proof.
+intros.
+remember (PointTermDepth x) as depth_x.
+induction depth_x.
+- symmetry in Heqdepth_x.
+ apply PointTermDepth_0 in Heqdepth_x.
+ subst x. 
+ case y.
+ intros; right; discriminate.
+ intros; right; discriminate.
+ intros; right; discriminate.
+ intros; right; discriminate.
+ intros; right; discriminate.
+ intros; right; discriminate.
+ left; congruence.
+-
+ case x.
+ case y.
+ intros.
+ apply Primitive_eq_dec.
+ right; discriminate.
+ right; discriminate.
+ right; discriminate.
+ right; discriminate.
+ right; discriminate.
+ right; discriminate.
+ case y.
+ right; discriminate.
+ intros.
+ apply Atom_eq_dec.
+ right; discriminate.
+ right; discriminate.
+ right; discriminate.
+ right; discriminate.
+ right; discriminate.
+ case y.
+ right; discriminate.
+ right; discriminate.
+ intros.
+ apply mt_pt_dec_prop.
+ 
+
+ right; discriminate.
+ right; discriminate.
+ right; discriminate.
+ right; discriminate.
+ right; discriminate.
+ right; discriminate.
+ right; discriminate.
+ right; discriminate.
+
+
+
+
+admit.
+apply list_eq_dec.
+apply pair_eq_dec.
+apply Name_eq_dec.
+apply pt_mt_dec_prop.
+admit.
+apply pt_mt_dec_prop.
+admit.
+apply pt_mt_dec_prop.
+Qed.
+
+
+Lemma pass_list:  (forall x y:MultiTerm, { x = y } + { x <> y}) -> forall x y: list MultiTerm, {x = y} + { x <> y}.
+Proof.
+intros.
+decide equality.
+Qed.
+
+
+
+(*
+Lemma unnorm_multiterm_eq_dec: forall x y:MultiTerm, { x = y } + {  x <> y }.
+Proof.
+ intros.
+ case x.
+Qed.
+*)
+
+
+Fixpoint unnorm_multiterm_eq (t: MultiTerm) (s: MultiTerm): bool  :=
+ match t with 
+  errorTerm msg => match s with
+                                  errorTerm msg1  => if (string_dec msg msg1)then true else false
+                                 | _  =>  false
+                               end
+  | point pt => match s with
+                      point st => unnorm_pointterm_eq pt st
+                      |_ => false
+                    end
+ | _ => false
+ end with unnorm_pointterm_eq (pt:PointTerm)(st:PointTerm):bool :=
+  match pt with
+    primitiveTerm pv => match st with 
+          primitiveTerm sv =>  if (PrimitiveValue_eq_dec pv sv) then true else false
+          | _ => false
+       end
+    | _ => false
+end.
+
+Definition IsSetTerm :=  { x: MultiTerm | exists sx: (list PointTerm),  x =  setTerm  sx }.
+
+
+Fixpoint setTermAdd (x: MultiTerm) (y:PointTerm): MultiTerm := 
+match x with
+  setTerm sx => match y with
+                             nilTerm => x
+                             | _ => if (set_In y sx) then sx else setTerm (set_add y sx)
+                         end
+ | point px => setTermAdd (setTerm [px]) y
+end
+.
+
 
 Fixpoint withScope (t:MultiTerm) (s:MultiTerm) : MultiTerm :=
-  match t with
+  match t wit
     | errorTerm msg => t 
     |  starTerm => scopedStarTerm s
     |  scopedStarTerm s1 => scopedStarTerm (ScopeAnd s s1)
-    |  setTerm ts => setTerm (map (fun x => withScopeP x s) ts) 
+    |  setTerm ts => setTerm (flat_map (fun x => setTerm withScopeP x s) ts) 
     |  point pt => point (withScopeP pt s)
   end with  withScopeP (t:PointTerm) (s: MultiTerm): PointTerm :=
       match t with 
@@ -76,9 +380,20 @@ Fixpoint withScope (t:MultiTerm) (s:MultiTerm) : MultiTerm :=
           | point pt => point( withScopeP pt t1)
           | errorTerm msg => errorTerm msg
           end
+       | setTerm ts => 
+            setTerm (map (fun x => ScopeAndP x s) ts)
        | _ => AtomTerm (StringName "TODO") 
-     end
-. 
+     end with ScopeAndP (t: PointTerm) (s: MultiTerm) : PointTerm =
+      match t with
+       primitiveTerm value =>  
+          match s with
+           starTerm => t
+           | point ps  =>  if (t = ps) then t else nilTerm
+           (*| _  => (atomTerm (StringName "TODO")) *)
+          end
+      |  _  => atomTerm (StringName "TODO")
+   end
+.
 
 
 
