core/scala/build.sbt
@@ -6,7 +6,8 @@ lazy val commonSettings = Seq(
   libraryDependencies ++= Seq(
     scalaVersion("org.scala-lang" % "scala-reflect" % _).value,
     "com.chuusai" %% "shapeless" % "2.3.2",
-    "org.typelevel" %% "cats" % "0.9.0",
+    "org.typelevel" %% "cats-core" % "1.0.0-MF",
+    "org.typelevel" %% "cats-effect" % "0.4",
     "com.typesafe.scala-logging" %% "scala-logging" % "3.5.0",
     "ch.qos.logback" % "logback-classic" % "1.1.7",
     "org.scalatest" %% "scalatest" % "3.0.1" % Test
